src/cbor/pulse/CBOR.Pulse.API.Nondet.C.fsti
@@ -1,0 +1,139 @@
+module CBOR.Pulse.API.Nondet.C
+include CBOR.Pulse.API.Nondet.Type
+open CBOR.Pulse.API.Base
+open Pulse.Lib.Pervasives
+
+module Spec = CBOR.Spec.API.Format
+module SZ = FStar.SizeT
+module U8 = FStar.UInt8
+module Trade = Pulse.Lib.Trade.Util
+module SM = Pulse.Lib.SeqMatch.Util
+
+val cbor_nondet_match: perm -> cbor_nondet_t -> Spec.cbor -> slprop
+
+inline_for_extraction noextract [@@noextract_to "krml"]
+val cbor_nondet_reset_perm (_: unit) : reset_perm_t #_ cbor_nondet_match
+
+val cbor_nondet_share
+  (_: unit)
+: CBOR.Pulse.API.Base.share_t u#0 u#0 #_ #_ cbor_nondet_match
+
+val cbor_nondet_gather
+  (_: unit)
+: CBOR.Pulse.API.Base.gather_t u#0 u#0 #_ #_ cbor_nondet_match
+
+val cbor_nondet_validate (_: unit) : cbor_nondet_validate_from_arrayptr_t
+
+val cbor_nondet_parse_valid (_: unit) : cbor_nondet_parse_valid_from_arrayptr_t #cbor_nondet_t cbor_nondet_match
+
+val cbor_nondet_serialize
+  (_: unit)
+: cbor_nondet_serialize_to_arrayptr_t #cbor_nondet_t cbor_nondet_match
+
+(* Destructors *)
+
+val cbor_nondet_major_type (_: unit) : get_major_type_t u#0 #_ cbor_nondet_match
+
+val cbor_nondet_read_simple_value (_: unit) : read_simple_value_t u#0 #_ cbor_nondet_match
+
+val cbor_nondet_elim_simple (_: unit) : elim_simple_t u#0 #_ cbor_nondet_match
+
+val cbor_nondet_read_uint64 (_: unit) : read_uint64_t u#0 #_ cbor_nondet_match
+
+val cbor_nondet_elim_int64 (_: unit) : elim_int64_t u#0 #_ cbor_nondet_match
+
+val cbor_nondet_get_string_length (_: unit) : get_string_length_t u#0 #_ cbor_nondet_match
+
+val cbor_nondet_get_string (_: unit) : get_string_as_arrayptr_t u#0 #_ cbor_nondet_match
+
+val cbor_nondet_get_tagged_tag (_: unit) : get_tagged_tag_t u#0 #_ cbor_nondet_match
+
+val cbor_nondet_get_tagged_payload (_: unit) : get_tagged_payload_t u#0 #_ cbor_nondet_match
+
+val cbor_nondet_get_array_length (_: unit) : get_array_length_t u#0 #_ cbor_nondet_match
+
+val cbor_nondet_array_iterator_match: perm -> cbor_nondet_array_iterator_t -> list Spec.cbor -> slprop
+
+val cbor_nondet_array_iterator_start (_: unit) : array_iterator_start_t u#0 u#0 #_ #_ cbor_nondet_match cbor_nondet_array_iterator_match
+
+val cbor_nondet_array_iterator_is_empty (_: unit) : array_iterator_is_empty_t u#0 #_ cbor_nondet_array_iterator_match
+
+val cbor_nondet_array_iterator_length (_: unit) : array_iterator_length_t u#0 #_ cbor_nondet_array_iterator_match
+
+val cbor_nondet_array_iterator_next (_: unit) : array_iterator_next_t u#0 #_ #_ cbor_nondet_match cbor_nondet_array_iterator_match
+
+val cbor_nondet_array_iterator_truncate (_: unit) : array_iterator_truncate_t u#0 #_ cbor_nondet_array_iterator_match
+
+val cbor_nondet_array_iterator_share (_: unit) : share_t u#0 u#0 #_ #_ cbor_nondet_array_iterator_match
+
+val cbor_nondet_array_iterator_gather (_: unit) : gather_t u#0 u#0 #_ #_ cbor_nondet_array_iterator_match
+
+val cbor_nondet_get_array_item (_: unit) : get_array_item_t u#0 #_ cbor_nondet_match
+
+val cbor_nondet_get_map_length (_: unit) : get_map_length_t u#0 #_ cbor_nondet_match
+
+val cbor_nondet_map_iterator_match: perm -> cbor_nondet_map_iterator_t -> list (Spec.cbor & Spec.cbor) -> slprop
+
+val cbor_nondet_map_iterator_start (_: unit) : map_iterator_start_t u#0 u#0 #_ #_ cbor_nondet_match cbor_nondet_map_iterator_match
+
+val cbor_nondet_map_iterator_is_empty (_: unit) : map_iterator_is_empty_t u#0 #_ cbor_nondet_map_iterator_match
+
+val cbor_nondet_map_entry_match: perm -> cbor_nondet_map_entry_t -> Spec.cbor & Spec.cbor -> slprop
+
+val cbor_nondet_map_iterator_next (_: unit) : map_iterator_next_t u#0 #_ #_ cbor_nondet_map_entry_match cbor_nondet_map_iterator_match
+
+val cbor_nondet_map_iterator_share (_: unit) : share_t u#0 u#0 #_ #_ cbor_nondet_map_iterator_match
+
+val cbor_nondet_map_iterator_gather (_: unit) : gather_t u#0 u#0 #_ #_ cbor_nondet_map_iterator_match
+
+val cbor_nondet_map_entry_key (_: unit) : map_entry_key_t u#0 u#0 #_ #_ cbor_nondet_map_entry_match cbor_nondet_match
+
+val cbor_nondet_map_entry_value (_: unit) : map_entry_value_t u#0 u#0 #_ #_ cbor_nondet_map_entry_match cbor_nondet_match
+
+val cbor_nondet_map_entry_share
+  (_: unit)
+: share_t u#0 u#0 #_ #_ cbor_nondet_map_entry_match
+
+val cbor_nondet_map_entry_gather
+  (_: unit)
+: gather_t u#0 u#0 #_ #_ cbor_nondet_map_entry_match
+
+(* Equality *)
+
+val cbor_nondet_equal
+  (x1: cbor_nondet_t)
+  (#p1: perm)
+  (#v1: Ghost.erased Spec.cbor)
+  (x2: cbor_nondet_t)
+  (#p2: perm)
+  (#v2: Ghost.erased Spec.cbor)
+: stt bool
+(requires
+  cbor_nondet_match p1 x1 v1 **
+  cbor_nondet_match p2 x2 v2
+)
+(ensures fun res ->
+  cbor_nondet_match p1 x1 v1 **
+  cbor_nondet_match p2 x2 v2 **
+  pure (res == true <==> Ghost.reveal v1 == Ghost.reveal v2)
+)
+
+val cbor_nondet_map_get (_: unit)
+: map_get_by_ref_t #_ cbor_nondet_match
+
+(* Constructors *)
+
+val cbor_nondet_mk_simple_value (_: unit) : mk_simple_t u#0 #_ cbor_nondet_match
+
+val cbor_nondet_mk_int64 (_: unit) : mk_int64_t u#0 #_ cbor_nondet_match
+
+val cbor_nondet_mk_string (_: unit) : mk_string_from_arrayptr_t u#0 #_ cbor_nondet_match
+
+val cbor_nondet_mk_tagged (_: unit) : mk_tagged_t #_ cbor_nondet_match
+
+val cbor_nondet_mk_array (_: unit) : mk_array_from_arrayptr_t #_ cbor_nondet_match
+
+val cbor_nondet_mk_map_entry (_: unit) : mk_map_entry_t #_ #_ cbor_nondet_match cbor_nondet_map_entry_match
+
+val cbor_nondet_mk_map_gen (_: unit)
+: mk_map_from_arrayptr_safe_t #cbor_nondet_t #cbor_nondet_map_entry_t cbor_nondet_match cbor_nondet_map_entry_match
